checker/coq/reif.v
@@ -7,12 +7,12 @@ Definition reified (C : Constraint) : Type :=
 Definition eval_reif (C : Constraint) (r : reified C) (theta : asg) :=
   (eval_lit (neglit (fst r)) theta) \/ C.(eval) (snd r) theta.
 
-Definition check_reif (C : Constraint) (r : reified C) (cl : clause) : bool :=
-  andb (check_clause (cons (neglit (fst r)) nil) cl) (C.(check) (snd r) cl).
-Theorem check_reif_valid : forall (C : Constraint) (r : reified C) (cl : clause),
-  check_reif C r cl = true -> implies (eval_reif C r) (eval_clause cl).
+Definition check_reif (C : Constraint) (Ch : Checker C) (r : reified C) (cl : clause) : bool :=
+  andb (check_clause (cons (neglit (fst r)) nil) cl) ((check C Ch) (snd r) cl).
+Theorem check_reif_valid : forall (C : Constraint) (Ch : Checker C) (r : reified C) (cl : clause),
+  check_reif C Ch r cl = true -> implies (eval_reif C r) (eval_clause cl).
 Proof.
-  unfold check_reif, implies, eval_reif. intros C r cl.
+  unfold check_reif, implies, eval_reif. intros C Ch r cl.
   rewrite andb_true_iff.
   intros.
   destruct H.
@@ -23,11 +23,13 @@ Proof.
   apply H0.
   unfold eval_clause. tauto.
 
-  assert (C.(check) (snd r) cl = true -> implies (C.(eval) (snd r)) (eval_clause cl)).
-  apply C.(check_valid).
+  assert ((check C Ch) (snd r) cl = true -> implies (C.(eval) (snd r)) (eval_clause cl)).
+  apply (check_valid C Ch).
   unfold implies in H0.
   apply H0. exact H1. exact Hc.
 Qed.
 
 Definition ReifiedConstraint (C : Constraint) : Constraint :=
-  mkConstraint (reified C) (eval_reif C) (check_reif C) (check_reif_valid C).
+  mkConstraint (reified C) (eval_reif C).
+Definition ReifiedCheck (C : Constraint) (Ch : Checker C) :=
+  mkChecker (ReifiedConstraint C) (check_reif C Ch) (check_reif_valid C Ch).
