checker/coq/map.v
@@ -1,5 +1,6 @@
 (* Module for dealing with maps. *)
 Require Import ZArith.
+Require ZArith.ZArith_dec.
 Require Import OrderedType.
 Require FSets.
 Require FSets.FMapAVL.
@@ -79,3 +80,93 @@ End Z_as_map_OT.
 Module ZMaps := FSets.FMapAVL.IntMake(Z_as_Int)(Z_as_map_OT).
 
 Definition zmap (T : Type) : Type := ZMaps.t T.
+
+Lemma find_mapsto_iff : forall (A : Type) (m :ZMaps.t A) x e, ZMaps.MapsTo x e m <-> ZMaps.find x m = Some e.
+Proof.
+  split; [apply ZMaps.find_1|apply ZMaps.find_2].
+Qed.
+
+(* Grabbed from a newer version of coq. *)
+Lemma eq_option_alt : forall (elt : Type) (o o' : option elt),
+  o = o' <-> (forall e, o=Some e <-> o' = Some e).
+Proof.
+  split; intros.
+  subst; split; auto.
+  destruct o; destruct o'; try rewrite H; auto.
+  symmetry; rewrite <- H; auto.
+Qed.
+
+Lemma not_find_in_iff : forall (A : Type) (m : ZMaps.t A) (x : ZMaps.key), ~ ZMaps.In x m <-> ZMaps.find x m = None.
+Proof.
+  split; intros.
+  rewrite eq_option_alt. intro e. rewrite <- find_mapsto_iff.
+  split; try discriminate. intro H'; elim H; exists e; auto.
+  intros (e,He).
+  assert (ZMaps.MapsTo x e m <-> ZMaps.find x m = Some e) as H'.
+    apply find_mapsto_iff.
+  unfold ZMaps.MapsTo in H'.
+  rewrite H in H'.
+  apply H' in He.
+  discriminate.
+Qed.
+
+Theorem find_empty_none : forall (A : Type) (x : ZMaps.key), ZMaps.find x (ZMaps.empty A) = None.
+Proof.
+  intros.
+  apply not_find_in_iff.
+  intros (e,Hc).
+  assert (ZMaps.Empty (ZMaps.empty A)).
+    apply ZMaps.empty_1.
+  unfold ZMaps.Empty, ZMaps.Raw.Proofs.Empty in H.
+  assert (~ ZMaps.Raw.MapsTo x e (ZMaps.this (ZMaps.empty A))).
+    apply H.
+  tauto.
+Qed.
+
+Theorem not_in_notmap : forall (A : Type) (xs : ZMaps.t A) (x  : ZMaps.key),
+  ~ ZMaps.In x xs <-> forall e, ~ ZMaps.MapsTo x e xs.
+  split; intros.
+    intro.
+      apply not_find_in_iff in H.
+      apply ZMaps.find_1 in H0. rewrite H in H0. discriminate.
+    apply not_find_in_iff.
+    apply eq_option_alt.
+    split; intros.
+      apply ZMaps.find_2 in H0.
+      now apply H in H0.
+
+      discriminate.
+Qed.
+
+Theorem find_add_none : forall (A : Type) (xs : ZMaps.t A) (x a : ZMaps.key) (e : A),
+  ZMaps.find a (ZMaps.add x e xs) = None <-> a <> x /\ ZMaps.find a xs = None.
+  split; intros.
+    split.
+      apply not_find_in_iff in H.
+      rewrite not_in_notmap in H.
+      intro.
+        assert (ZMaps.MapsTo a e (ZMaps.add x e xs)).
+          rewrite H0.  now apply ZMaps.add_1.
+        now apply H in H1.
+
+        apply not_find_in_iff.
+        apply not_find_in_iff in H.
+        rewrite not_in_notmap in H.
+        apply not_in_notmap; intros.
+        assert ({x = a} + {x <> a}). apply ZArith.ZArith_dec.Z_eq_dec.
+        destruct H0 as [H0 | H0]; intros; intro.
+          assert (ZMaps.MapsTo a e (ZMaps.add x e xs)).
+            rewrite H0; now apply ZMaps.add_1. now apply H in H2.
+          assert (ZMaps.MapsTo a e0 (ZMaps.add x e xs)).
+            apply ZMaps.add_2. assumption. assumption.
+            now apply H in H2.
+    destruct H as [Hne Hnf].
+    apply eq_option_alt; split; intros.
+      apply not_find_in_iff in Hnf; rewrite not_in_notmap in Hnf.
+      assert (ZMaps.MapsTo a e0 xs).
+        apply ZMaps.add_3 with (x := x) (e' := e).
+          congruence.
+          now apply ZMaps.find_2.
+          now apply Hnf in H0.
+        discriminate.
+Qed.
