checker/coq/sol.v
@@ -1,0 +1,37 @@
+(* Stuff for dealing with solutions. *)(* Computing domains/bounds from the complement of a clause. *)
+Require Import ZArith.
+Require Import Bool.
+Require Import List.
+Require Import FSets.FMapFacts.
+Require Import zset.
+Require Import map.
+Require Import prim.
+Require Import bounds.
+Require Import domain.
+
+(* Partial solution - mapping of variables to integers. *)
+Definition zsol : Type := zmap Z.
+
+Definition eval_zsol zs theta :=
+  forall (x : ivar) (v : Z),
+    ZMaps.MapsTo x v zs -> eval_ivar x theta = v.
+
+Definition zsol_val (zs : zsol) (x : ivar) :=
+  ZMaps.find x zs.
+
+Lemma zsol_val_valid : forall (zs : zsol) (x : ivar) (v : Z),
+  zsol_val zs x = Some v ->
+    forall theta, eval_zsol zs theta -> eval_ivar x theta = v.
+Proof.
+  intros zs x v; unfold zsol_val; intros.
+  unfold eval_zsol in H0.
+  now apply ZMaps.find_2, H0 in H.
+Qed.
+
+Record SolCheck (C : Constraint) := mkSolCheck
+  {
+    sol_check : C.(T) -> zsol -> bool ;
+    sol_check_valid : forall (x : C.(T) ) (zs : zsol),
+      (sol_check x zs = true) ->
+        implies (eval_zsol zs) (C.(eval) x)
+  }.
